applicative-intersection-no-typing-stack/Proof/Consistent.v
@@ -1,0 +1,44 @@
+Require Import Metalib.Metatheory.
+Require Import Coq.Program.Equality.
+Require Import Language LibTactics.
+Require Import Tred.
+
+Theorem consistent_soundness :
+  forall (v1 v2 : trm) (A B : typ),
+    value v1 -> value v2 ->
+    typing nil v1 A ->
+    typing nil v2 B ->
+    consistent v1 v2 ->
+    consistency_spec v1 v2.
+Proof.
+  introv Hv1 Hv2 Htyp1 Htyp2 Hcons.
+  unfold consistency_spec.
+  intros C v1' v2' Hord Htred1 Htred2.
+  eapply tred_determinism.
+  eapply Hv1. eapply Hv2. eapply Htyp1. eapply Htyp2.
+  eapply Htred1. eapply Htred2. assumption.
+Qed.
+
+Ltac ind_exp_size s :=
+  assert (SizeInd: exists i, s < i) by eauto;
+  destruct SizeInd as [i SizeInd];
+  repeat match goal with | [ h : trm |- _ ] => (gen h) end;
+  induction i as [|i IH]; [
+      intros; match goal with | [ H : _ < 0 |- _ ] => (dependent destruction H; eauto) end
+    | intros ].
+
+Theorem consistent_completeness :
+  forall (v1 v2 : trm) (A B : typ),
+    value v1 -> value v2 ->
+    typing nil v1 A ->
+    typing nil v2 B ->
+    consistency_spec v1 v2 ->
+    consistent v1 v2.
+Proof.
+  introv Hv1 Hv2 Htyp1 Htyp2 Hcons.
+  gen Hv1 Hv2 Hcons A B.
+  ind_exp_size (size_trm v1 + size_trm v2).
+  dependent destruction Hv1; dependent destruction Hv2; eauto.
+  - dependent destruction H; dependent destruction H0.
+    + eapply tred_progress in Htyp1; eauto.
+Abort.
