applicative-intersection-no-typing-stack/Proof/Disjoint.v
@@ -3,3 +3,77 @@ Require Import Coq.Program.Equality.
 Require Import Language LibTactics.
 Require Import Strings.String.
 Require Import Program.Tactics.
+Require Import SubAndTopLike.
+Require Import Psatz. (* lia *)
+
+Ltac ind_typ_size s :=
+  assert (SizeInd: exists i, s < i) by eauto;
+  destruct SizeInd as [i SizeInd];
+  repeat match goal with
+         | [ h : typ |- _ ] => (gen h)
+         end;
+  induction i as [|i IH]; [
+      intros; match goal with
+              | [ H : _ < 0 |- _ ] => (dependent destruction H)
+              end
+    | intros ].
+
+Lemma split_decrease_size:
+  forall A B C,
+    splitable A B C -> size_typ B < size_typ A /\ size_typ C < size_typ A.
+Proof.
+  introv H. dependent induction H; simpl; lia.
+Qed.
+
+Theorem disjoint_complete :
+  forall A B, disjoint A B -> disjoint_spec A B.
+Proof.
+  intros A B Hdisj C Hsub1 Hsub2.
+  ind_typ_size (size_typ A + size_typ B + size_typ C).
+  destruct (split_or_ord C).
+  - dependent destruction Hdisj; try solve [eapply sub_toplike_preservation; eauto 3].
+    + dependent destruction Hsub1.
+      * eapply sub_toplike_preservation; eauto.
+      * exfalso. eapply split_and_ord; eauto.
+      * simpl in SizeInd.
+        assert ((size_typ A1 + size_typ B + size_typ C) < i) by lia.
+        now pose proof (IH _ _ Hdisj1 _ Hsub1 Hsub2 H1).
+      * simpl in SizeInd.
+        assert ((size_typ A2 + size_typ B + size_typ C) < i) by lia.
+        now pose proof (IH _ _ Hdisj2 _ Hsub1 Hsub2 H1).
+    + dependent destruction Hsub2.
+      * eapply sub_toplike_preservation; eauto.
+      * exfalso. eapply split_and_ord; eauto.
+      * simpl in SizeInd.
+        assert ((size_typ A + size_typ B1 + size_typ C) < i) by lia.
+        now pose proof (IH _ _ Hdisj1 _ Hsub1 Hsub2 H1).
+      * simpl in SizeInd.
+        assert ((size_typ A + size_typ B2 + size_typ C) < i) by lia.
+        now pose proof (IH _ _ Hdisj2 _ Hsub1 Hsub2 H1).
+    + dependent destruction Hsub1; dependent destruction Hsub2; eauto 3.
+      * inversion H.
+      * dependent destruction H.
+        exfalso. eapply split_and_ord; eauto.
+      * exfalso. eapply split_and_ord; eauto.
+    + dependent destruction Hsub1; dependent destruction Hsub2; eauto 3.
+      * exfalso. eapply split_and_ord; eauto.
+      * inversion H.
+      * exfalso. eapply split_and_ord; eauto.
+    + dependent destruction Hsub1; dependent destruction Hsub2; eauto 3.
+      * constructor. eapply IH.
+        eapply Hdisj. eapply Hsub1_2. eapply Hsub2_2.
+        simpl in SizeInd. lia.
+      * exfalso. eapply split_and_ord; eauto.
+      * exfalso. eapply split_and_ord; eauto.
+      * exfalso. eapply split_and_ord; eauto.
+  - destruct_conjs.
+    dependent destruction Hsub1; dependent destruction Hsub2;
+      try solve [exfalso; eapply split_and_ord; eauto].
+    eapply split_determinism in H0; eauto 3. destruct_conjs. subst.
+    eapply split_determinism in H; eauto 3. destruct_conjs. subst.
+    pose proof (split_decrease_size _ _ _ H3).
+    destruct_conjs.
+    eapply toplike_spl_combine; eauto 3.
+    + eapply IH; eauto 3. lia.
+    + eapply IH; eauto 3. lia.
+Qed.
